Refactoring and unifying names

txn-data-consistency/CCv_Eiger_Port_plus.thy
@@ -8,21 +8,21 @@ section \<open>Event system & Refinement from ET_ES to tps\<close>
 
 subsection \<open>State\<close>
 
-type_synonym svr_id = key
+type_synonym key = key
 type_synonym tstmp = nat
 type_synonym dep_set = "(key \<times> txid) set"
 
 \<comment> \<open>Client State\<close>
-datatype 'v state_txn =
+datatype 'v txn_state =
   Idle | RtxnInProg "key set" "key \<rightharpoonup> ('v \<times> txid)" | WtxnPrep "key \<rightharpoonup> 'v" | WtxnCommit tstmp "key \<rightharpoonup> 'v" dep_set
 
-record 'v client =
-  txn_state :: "'v state_txn"
-  txn_sn :: sqn
-  gst :: tstmp
-  lst_map :: "svr_id \<Rightarrow> tstmp"
-  cl_ctx :: dep_set \<comment> \<open>history variable\<close>
+record 'v cl_conf =
+  cl_state :: "'v txn_state"
+  cl_sn :: sqn
   cl_clock :: tstmp
+  cl_ctx :: dep_set \<comment> \<open>history variable\<close>
+  gst :: tstmp
+  lst_map :: "key \<Rightarrow> tstmp"
 
 definition dep_set_init :: dep_set where
   "dep_set_init \<equiv> \<Union>k. {(k, T0)}"
@@ -39,34 +39,34 @@ fun is_prepared :: "'v ver_state \<Rightarrow> bool" where
   "is_prepared (Prep _ _) = True" |
   "is_prepared _ = False"
 
-type_synonym 'v state_wtxn = "txid \<Rightarrow> 'v ver_state"
+type_synonym 'v wtxn_state = "txid \<Rightarrow> 'v ver_state"
 
-record 'v server =
-  wtxn_state :: "'v state_wtxn"
-  clock :: tstmp
+record 'v svr_conf =
+  svr_state :: "'v wtxn_state"
+  svr_clock :: tstmp
   lst :: tstmp
 
-abbreviation wtxns_emp :: "'v state_wtxn" where
+abbreviation wtxns_emp :: "txid \<Rightarrow> 'v ver_state" where
   "wtxns_emp \<equiv> (\<lambda>t. No_Ver)"
 
 \<comment> \<open>Global State\<close>
-record 'v state = 
-  cls :: "cl_id \<Rightarrow> 'v client"
-  svrs :: "svr_id \<Rightarrow> 'v server"
-  commit_order :: "key \<Rightarrow> txid list"
-  \<comment> \<open>history variable: order of client commit for write transactions\<close>
+record 'v global_conf = 
+  cls :: "cl_id \<Rightarrow> 'v cl_conf"
+  svrs :: "key \<Rightarrow> 'v svr_conf"
   rtxn_rts :: "txid0 \<rightharpoonup> tstmp"
   wtxn_cts :: "txid \<rightharpoonup> tstmp"
+  commit_order :: "key \<Rightarrow> txid list"
+  \<comment> \<open>history variable: order of client commit for write transactions\<close>
 
 
 subsection \<open>Functions\<close>
 
 subsubsection \<open>Translator functions\<close>
 
-abbreviation get_txn :: "'v state \<Rightarrow> cl_id \<Rightarrow> txid0" where
-  "get_txn s cl \<equiv> Tn_cl (txn_sn (cls s cl)) cl"
+abbreviation get_txn :: "'v global_conf \<Rightarrow> cl_id \<Rightarrow> txid0" where
+  "get_txn s cl \<equiv> Tn_cl (cl_sn (cls s cl)) cl"
 
-abbreviation get_wtxn :: "'v state \<Rightarrow> cl_id \<Rightarrow> txid" where
+abbreviation get_wtxn :: "'v global_conf \<Rightarrow> cl_id \<Rightarrow> txid" where
   "get_wtxn s cl \<equiv> Tn (get_txn s cl)"
 
 fun get_cl_w :: "txid \<Rightarrow> cl_id" where
@@ -83,15 +83,15 @@ fun get_rs :: "'v ver_state \<Rightarrow> txid0 set" where
   "get_rs (Commit _ _ rs _) = rs"
 
 
-subsubsection \<open>Customised dom and ran functions for wtxn_state\<close>
+subsubsection \<open>Customised dom and ran functions for svr_state\<close>
 
-definition wtxns_dom :: "'v state_wtxn \<Rightarrow> txid set" where
+definition wtxns_dom :: "'v wtxn_state \<Rightarrow> txid set" where
   "wtxns_dom wtxns \<equiv> {t. wtxns t \<noteq> No_Ver}"
 
-definition wtxns_vran :: "'v state_wtxn \<Rightarrow> 'v set" where
+definition wtxns_vran :: "'v wtxn_state \<Rightarrow> 'v set" where
   "wtxns_vran wtxns \<equiv> {get_val (wtxns t) | t. t \<in> wtxns_dom wtxns}"
 
-definition wtxns_rsran :: "'v state_wtxn \<Rightarrow> txid0 set" where
+definition wtxns_rsran :: "'v wtxn_state \<Rightarrow> txid0 set" where
   "wtxns_rsran wtxns \<equiv> \<Union>{get_rs (wtxns t) | t. t \<in> wtxns_dom wtxns}"
 
 
@@ -114,16 +114,16 @@ definition ver_committed_after :: "'v ver_state \<Rightarrow> tstmp \<Rightarrow
 
 
 \<comment> \<open>returns the writer transaction id of the version read at read timestamp (highest cts less than ts)\<close>
-definition at :: "'v state_wtxn \<Rightarrow> tstmp \<Rightarrow> txid" where 
+definition at :: "'v wtxn_state \<Rightarrow> tstmp \<Rightarrow> txid" where 
   "at wtxns rts = (ARG_MAX (get_ts o wtxns) t. ver_committed_before (wtxns t) rts)"
 
-definition newest_own_write :: "'v state_wtxn \<Rightarrow> tstmp \<Rightarrow> cl_id \<rightharpoonup> txid" where
+definition newest_own_write :: "'v wtxn_state \<Rightarrow> tstmp \<Rightarrow> cl_id \<rightharpoonup> txid" where
   "newest_own_write wtxns ts cl = 
      (if \<exists>t. ver_committed_after (wtxns t) ts \<and> get_cl_w t = cl
      then Some (ARG_MAX (get_ts o wtxns) t. ver_committed_after (wtxns t) ts \<and> get_cl_w t = cl)
      else None)"
 
-definition read_at :: "'v state_wtxn \<Rightarrow> tstmp \<Rightarrow> cl_id \<Rightarrow> txid" where
+definition read_at :: "'v wtxn_state \<Rightarrow> tstmp \<Rightarrow> cl_id \<Rightarrow> txid" where
   "read_at wtxns ts cl \<equiv> let t = at wtxns ts in
     (case newest_own_write wtxns (get_ts (wtxns t)) cl of
       None \<Rightarrow> t |
@@ -132,22 +132,22 @@ definition read_at :: "'v state_wtxn \<Rightarrow> tstmp \<Rightarrow> cl_id \<R
 
 subsubsection \<open>Helper functions\<close>
 
-definition add_to_readerset :: "'v state_wtxn \<Rightarrow> txid0 \<Rightarrow> txid \<Rightarrow> 'v state_wtxn" where
+definition add_to_readerset :: "'v wtxn_state \<Rightarrow> txid0 \<Rightarrow> txid \<Rightarrow> 'v wtxn_state" where
   "add_to_readerset wtxns t t_wr \<equiv> (case wtxns t_wr of
     Commit cts v rs deps \<Rightarrow> wtxns (t_wr := Commit cts v (insert t rs) deps) |
     _ \<Rightarrow> wtxns)"
 
-definition pending_wtxns_ts :: "'v state_wtxn \<Rightarrow> tstmp set" where
+definition pending_wtxns_ts :: "'v wtxn_state \<Rightarrow> tstmp set" where
   "pending_wtxns_ts wtxns \<equiv> {prep_t. \<exists>t v. wtxns t = Prep prep_t v}"
 
-definition get_view :: "'v state \<Rightarrow> cl_id \<Rightarrow> dep_set" where
+definition get_view :: "'v global_conf \<Rightarrow> cl_id \<Rightarrow> dep_set" where
   "get_view s cl \<equiv> {(k, t). 
-    \<exists>cts v rs deps. wtxn_state (svrs s k) t = Commit cts v rs deps \<and>
+    \<exists>cts v rs deps. svr_state (svrs s k) t = Commit cts v rs deps \<and>
     (cts \<le> gst (cls s cl) \<or> get_cl_w t = cl)}"
 
-definition get_ctx :: "'v state \<Rightarrow> (key \<rightharpoonup> ('v \<times> txid)) \<Rightarrow> dep_set" where
+definition get_ctx :: "'v global_conf \<Rightarrow> (key \<rightharpoonup> ('v \<times> txid)) \<Rightarrow> dep_set" where
   "get_ctx s kvt_map \<equiv> \<Union>{insert (k, t) deps | k t deps.
-    \<exists>cts v rs. wtxn_state (svrs s k) t = Commit cts v rs deps \<and>
+    \<exists>cts v rs. svr_state (svrs s k) t = Commit cts v rs deps \<and>
     kvt_map k = Some (v, t)}"
 
 definition view_of :: "(key \<Rightarrow> txid list) \<Rightarrow> dep_set \<Rightarrow> view" where
@@ -160,169 +160,169 @@ subsection \<open>Events\<close>
 datatype 'v ev =
   RInvoke cl_id "key set" | Read cl_id key 'v txid | RDone cl_id "key \<rightharpoonup> ('v \<times> txid)" sqn view |
   WInvoke cl_id "key \<rightharpoonup> 'v" | WCommit cl_id "key \<rightharpoonup> 'v" tstmp sqn view | WDone cl_id "key \<rightharpoonup> 'v" |
-  RegR svr_id txid0 txid tstmp | PrepW svr_id txid 'v | CommitW svr_id txid 'v tstmp dep_set | Skip2
+  RegR key txid0 txid tstmp | PrepW key txid 'v | CommitW key txid 'v tstmp dep_set | Skip2
 
-abbreviation is_curr_t :: "'v state \<Rightarrow> txid0 \<Rightarrow> bool" where
-  "is_curr_t s t \<equiv> txn_sn (cls s (get_cl t)) = get_sn t"
+abbreviation is_curr_t :: "'v global_conf \<Rightarrow> txid0 \<Rightarrow> bool" where
+  "is_curr_t s t \<equiv> cl_sn (cls s (get_cl t)) = get_sn t"
 
-abbreviation is_curr_wt :: "'v state \<Rightarrow> txid \<Rightarrow> bool" where
-  "is_curr_wt s t \<equiv> t \<noteq> T0 \<and> txn_sn (cls s (get_cl_w t)) = get_sn_w t"
+abbreviation is_curr_wt :: "'v global_conf \<Rightarrow> txid \<Rightarrow> bool" where
+  "is_curr_wt s t \<equiv> t \<noteq> T0 \<and> cl_sn (cls s (get_cl_w t)) = get_sn_w t"
 
 
 subsubsection \<open>Client Events\<close>
 
-definition read_invoke :: "cl_id \<Rightarrow> key set \<Rightarrow> 'v state \<Rightarrow> 'v state \<Rightarrow> bool" where
+definition read_invoke :: "cl_id \<Rightarrow> key set \<Rightarrow> 'v global_conf \<Rightarrow> 'v global_conf \<Rightarrow> bool" where
   "read_invoke cl keys s s' \<equiv>
     keys \<noteq> {} \<and>
     finite keys \<and>
-    txn_state (cls s cl) = Idle \<and>
+    cl_state (cls s cl) = Idle \<and>
     s' = s \<lparr> cls := (cls s)
       (cl := cls s cl \<lparr>
-        txn_state := RtxnInProg keys Map.empty,
-        gst := Min (range (lst_map (cls s cl))),
-        cl_clock := Suc (cl_clock (cls s cl))
+        cl_state := RtxnInProg keys Map.empty,
+        cl_clock := Suc (cl_clock (cls s cl)),
+        gst := Min (range (lst_map (cls s cl)))
       \<rparr>)
     \<rparr>"
 
-definition read :: "cl_id \<Rightarrow> key \<Rightarrow> 'v \<Rightarrow> txid \<Rightarrow> 'v state \<Rightarrow> 'v state \<Rightarrow> bool" where
+definition read :: "cl_id \<Rightarrow> key \<Rightarrow> 'v \<Rightarrow> txid \<Rightarrow> 'v global_conf \<Rightarrow> 'v global_conf \<Rightarrow> bool" where
   "read cl k v t s s' \<equiv> 
-    \<comment> \<open>reads server k's value v for client transaction, lst, and clock\<close>
-    (\<exists>cts rs deps. wtxn_state (svrs s k) t = Commit cts v rs deps \<and> get_txn s cl \<in> rs) \<and>
-    (\<exists>keys kvt_map. txn_state (cls s cl) = RtxnInProg keys kvt_map \<and> k \<in> keys \<and> kvt_map k = None) \<and>
+    \<comment> \<open>reads server k's value v for client transaction, lst, and svr_clock\<close>
+    (\<exists>cts rs deps. svr_state (svrs s k) t = Commit cts v rs deps \<and> get_txn s cl \<in> rs) \<and>
+    (\<exists>keys kvt_map. cl_state (cls s cl) = RtxnInProg keys kvt_map \<and> k \<in> keys \<and> kvt_map k = None) \<and>
     s' = s \<lparr> cls := (cls s)
       (cl := cls s cl \<lparr>
-        txn_state :=
-          (case txn_state (cls s cl) of RtxnInProg keys kvt_map \<Rightarrow> RtxnInProg keys (kvt_map (k \<mapsto> (v, t)))),
-        lst_map := (lst_map (cls s cl)) (k := lst (svrs s k)),
-        cl_clock := Suc (max (cl_clock (cls s cl)) (clock (svrs s k)))
+        cl_state :=
+          (case cl_state (cls s cl) of RtxnInProg keys kvt_map \<Rightarrow> RtxnInProg keys (kvt_map (k \<mapsto> (v, t)))),
+        cl_clock := Suc (max (cl_clock (cls s cl)) (svr_clock (svrs s k))),
+        lst_map := (lst_map (cls s cl)) (k := lst (svrs s k))
       \<rparr>)
     \<rparr>"
 
-definition read_done :: "cl_id \<Rightarrow> (key \<rightharpoonup> ('v \<times> txid)) \<Rightarrow> sqn \<Rightarrow> view \<Rightarrow> 'v state \<Rightarrow> 'v state \<Rightarrow> bool" where
+definition read_done :: "cl_id \<Rightarrow> (key \<rightharpoonup> ('v \<times> txid)) \<Rightarrow> sqn \<Rightarrow> view \<Rightarrow> 'v global_conf \<Rightarrow> 'v global_conf \<Rightarrow> bool" where
   "read_done cl kvt_map sn u'' s s' \<equiv>
-    sn = txn_sn (cls s cl) \<and>
+    sn = cl_sn (cls s cl) \<and>
     u'' = view_of (commit_order s) (cl_ctx (cls s cl) \<union> get_ctx s kvt_map) \<and>
-    txn_state (cls s cl) = RtxnInProg (dom kvt_map) kvt_map \<and>
+    cl_state (cls s cl) = RtxnInProg (dom kvt_map) kvt_map \<and>
     s' = s \<lparr> cls := (cls s)
       (cl := cls s cl \<lparr>
-        txn_state := Idle,
-        txn_sn := Suc (txn_sn (cls s cl)),
-        cl_ctx := cl_ctx (cls s cl) \<union> get_ctx s kvt_map,
-        cl_clock := Suc (cl_clock (cls s cl))
+        cl_state := Idle,
+        cl_sn := Suc (cl_sn (cls s cl)),
+        cl_clock := Suc (cl_clock (cls s cl)),
+        cl_ctx := cl_ctx (cls s cl) \<union> get_ctx s kvt_map
       \<rparr>),
       rtxn_rts := (rtxn_rts s) (get_txn s cl \<mapsto> gst (cls s cl))
     \<rparr>"
 
-definition write_invoke :: "cl_id \<Rightarrow> (key \<rightharpoonup> 'v) \<Rightarrow> 'v state \<Rightarrow> 'v state \<Rightarrow> bool" where
+definition write_invoke :: "cl_id \<Rightarrow> (key \<rightharpoonup> 'v) \<Rightarrow> 'v global_conf \<Rightarrow> 'v global_conf \<Rightarrow> bool" where
   "write_invoke cl kv_map s s' \<equiv> 
     kv_map \<noteq> Map.empty \<and>
     finite (dom kv_map) \<and>
-    txn_state (cls s cl) = Idle \<and>
+    cl_state (cls s cl) = Idle \<and>
     s' = s \<lparr> cls := (cls s)
       (cl := cls s cl \<lparr>
-        txn_state := WtxnPrep kv_map,
+        cl_state := WtxnPrep kv_map,
         cl_clock := Suc (cl_clock (cls s cl))
       \<rparr>)
     \<rparr>"
 
-definition write_commit :: "cl_id \<Rightarrow> (key \<rightharpoonup> 'v) \<Rightarrow> tstmp \<Rightarrow> sqn \<Rightarrow> view \<Rightarrow> 'v state \<Rightarrow> 'v state \<Rightarrow> bool" where
+definition write_commit :: "cl_id \<Rightarrow> (key \<rightharpoonup> 'v) \<Rightarrow> tstmp \<Rightarrow> sqn \<Rightarrow> view \<Rightarrow> 'v global_conf \<Rightarrow> 'v global_conf \<Rightarrow> bool" where
   "write_commit cl kv_map commit_t sn u'' s s' \<equiv>
-    sn = txn_sn (cls s cl) \<and>            \<comment> \<open>@{term sn} needed in mediator function, not in event\<close>
+    sn = cl_sn (cls s cl) \<and>            \<comment> \<open>@{term sn} needed in mediator function, not in event\<close>
     u'' = view_of (commit_order s) (cl_ctx (cls s cl)) \<and>
-    txn_state (cls s cl) = WtxnPrep kv_map \<and>
-    (\<forall>k \<in> dom kv_map. is_prepared (wtxn_state (svrs s k) (get_wtxn s cl))) \<and>  \<comment> \<open>v = the (kv_map k)\<close>
-    commit_t = Max {get_ts (wtxn_state (svrs s k) (get_wtxn s cl)) | k. k \<in> dom kv_map} \<and>
+    cl_state (cls s cl) = WtxnPrep kv_map \<and>
+    (\<forall>k \<in> dom kv_map. is_prepared (svr_state (svrs s k) (get_wtxn s cl))) \<and>  \<comment> \<open>v = the (kv_map k)\<close>
+    commit_t = Max {get_ts (svr_state (svrs s k) (get_wtxn s cl)) | k. k \<in> dom kv_map} \<and>
 
     s' = s \<lparr> cls := (cls s)
       (cl := cls s cl \<lparr>
-        txn_state := WtxnCommit commit_t kv_map (cl_ctx (cls s cl)),
-        cl_ctx := cl_ctx (cls s cl) \<union> (\<Union>k \<in> dom kv_map. {(k, get_wtxn s cl)}),
-        cl_clock := Suc (max (cl_clock (cls s cl)) commit_t) \<comment> \<open>Why not max of all involved server clocks\<close>
+        cl_state := WtxnCommit commit_t kv_map (cl_ctx (cls s cl)),
+        cl_clock := Suc (max (cl_clock (cls s cl)) commit_t), \<comment> \<open>Why not max of all involved server svr_clocks\<close>
+        cl_ctx := cl_ctx (cls s cl) \<union> (\<Union>k \<in> dom kv_map. {(k, get_wtxn s cl)})
       \<rparr>), 
+      wtxn_cts := (wtxn_cts s) (get_wtxn s cl \<mapsto> commit_t),
       commit_order :=
-        (\<lambda>k. if kv_map k = None then commit_order s k else commit_order s k @ [get_wtxn s cl]),
-      wtxn_cts := (wtxn_cts s) (get_wtxn s cl \<mapsto> commit_t)
+        (\<lambda>k. if kv_map k = None then commit_order s k else commit_order s k @ [get_wtxn s cl])
     \<rparr>"
 
-definition write_done :: "cl_id \<Rightarrow> (key \<rightharpoonup> 'v) \<Rightarrow> 'v state \<Rightarrow> 'v state \<Rightarrow> bool" where
+definition write_done :: "cl_id \<Rightarrow> (key \<rightharpoonup> 'v) \<Rightarrow> 'v global_conf \<Rightarrow> 'v global_conf \<Rightarrow> bool" where
   "write_done cl kv_map s s' \<equiv>
-    (\<exists>cts ctx. txn_state (cls s cl) = WtxnCommit cts kv_map ctx \<and>
-      (\<forall>k\<in>dom kv_map. \<exists>v rs. wtxn_state (svrs s k) (get_wtxn s cl) = Commit cts v rs ctx)) \<and> \<comment> \<open>v = the (kv_map k)\<close>
+    (\<exists>cts ctx. cl_state (cls s cl) = WtxnCommit cts kv_map ctx \<and>
+      (\<forall>k\<in>dom kv_map. \<exists>v rs. svr_state (svrs s k) (get_wtxn s cl) = Commit cts v rs ctx)) \<and> \<comment> \<open>v = the (kv_map k)\<close>
     s' = s \<lparr> cls := (cls s)
       (cl := cls s cl \<lparr>
-        txn_state := Idle,
-        txn_sn := Suc (txn_sn (cls s cl)),
-        lst_map := (\<lambda>k. if kv_map k = None then lst_map (cls s cl) k else lst (svrs s k)),
-        cl_clock := Suc (max (cl_clock (cls s cl)) (Max {clock (svrs s k) | k. k \<in> dom kv_map}))
+        cl_state := Idle,
+        cl_sn := Suc (cl_sn (cls s cl)),
+        cl_clock := Suc (max (cl_clock (cls s cl)) (Max {svr_clock (svrs s k) | k. k \<in> dom kv_map})),
+        lst_map := (\<lambda>k. if kv_map k = None then lst_map (cls s cl) k else lst (svrs s k))
       \<rparr>)
     \<rparr>"
 
 
 subsubsection \<open>Server Events\<close>
 
-definition register_read :: "svr_id \<Rightarrow> txid0 \<Rightarrow> txid \<Rightarrow> tstmp \<Rightarrow> 'v state \<Rightarrow> 'v state \<Rightarrow> bool" where
+definition register_read :: "key \<Rightarrow> txid0 \<Rightarrow> txid \<Rightarrow> tstmp \<Rightarrow> 'v global_conf \<Rightarrow> 'v global_conf \<Rightarrow> bool" where
   "register_read svr t t_wr gst_ts s s' \<equiv>
     is_curr_t s t \<and>
-    (\<exists>keys kv_map. txn_state (cls s (get_cl t)) = RtxnInProg keys kv_map \<and> svr \<in> keys \<and> kv_map svr = None) \<and>
+    (\<exists>keys kv_map. cl_state (cls s (get_cl t)) = RtxnInProg keys kv_map \<and> svr \<in> keys \<and> kv_map svr = None) \<and>
     gst_ts = gst (cls s (get_cl t)) \<and>
-    t_wr = read_at (wtxn_state (svrs s svr)) gst_ts (get_cl t) \<and>
+    t_wr = read_at (svr_state (svrs s svr)) gst_ts (get_cl t) \<and>
     s' = s \<lparr> svrs := (svrs s)
       (svr := svrs s svr \<lparr>
-        wtxn_state := add_to_readerset (wtxn_state (svrs s svr)) t t_wr,
-        clock := Suc (max (clock (svrs s svr)) (cl_clock (cls s (get_cl t))))
+        svr_state := add_to_readerset (svr_state (svrs s svr)) t t_wr,
+        svr_clock := Suc (max (svr_clock (svrs s svr)) (cl_clock (cls s (get_cl t))))
       \<rparr>)
     \<rparr>"
 
-definition prepare_write :: "svr_id \<Rightarrow> txid \<Rightarrow> 'v \<Rightarrow> 'v state \<Rightarrow> 'v state \<Rightarrow> bool" where
+definition prepare_write :: "key \<Rightarrow> txid \<Rightarrow> 'v \<Rightarrow> 'v global_conf \<Rightarrow> 'v global_conf \<Rightarrow> bool" where
   "prepare_write svr t v s s' \<equiv>
     is_curr_wt s t \<and>
     \<comment> \<open>get client's value v for svr and cl_clock\<close>
     (\<exists>kv_map.
-      txn_state (cls s (get_cl_w t)) = WtxnPrep kv_map \<and> kv_map svr = Some v) \<and>
-    wtxn_state (svrs s svr) t = No_Ver \<and>
+      cl_state (cls s (get_cl_w t)) = WtxnPrep kv_map \<and> kv_map svr = Some v) \<and>
+    svr_state (svrs s svr) t = No_Ver \<and>
     s' = s \<lparr> svrs := (svrs s)
       (svr := svrs s svr \<lparr>
-        wtxn_state := (wtxn_state (svrs s svr))(t := Prep (clock (svrs s svr)) v),
-        clock := Suc (max (clock (svrs s svr)) (cl_clock (cls s (get_cl_w t)))) 
+        svr_state := (svr_state (svrs s svr))(t := Prep (svr_clock (svrs s svr)) v),
+        svr_clock := Suc (max (svr_clock (svrs s svr)) (cl_clock (cls s (get_cl_w t)))) 
       \<rparr>)
     \<rparr>"
 
-definition commit_write :: "svr_id \<Rightarrow> txid \<Rightarrow> 'v \<Rightarrow> tstmp \<Rightarrow> dep_set \<Rightarrow> 'v state \<Rightarrow> 'v state \<Rightarrow> bool" where
+definition commit_write :: "key \<Rightarrow> txid \<Rightarrow> 'v \<Rightarrow> tstmp \<Rightarrow> dep_set \<Rightarrow> 'v global_conf \<Rightarrow> 'v global_conf \<Rightarrow> bool" where
   "commit_write svr t v cts deps s s' \<equiv>
     is_curr_wt s t \<and>
-    (\<exists>kv_map. txn_state (cls s (get_cl_w t)) = WtxnCommit cts kv_map deps \<and> svr \<in> dom kv_map) \<and>
-    is_prepared (wtxn_state (svrs s svr) t) \<and> 
-    v = get_val (wtxn_state (svrs s svr) t) \<and>
+    (\<exists>kv_map. cl_state (cls s (get_cl_w t)) = WtxnCommit cts kv_map deps \<and> svr \<in> dom kv_map) \<and>
+    is_prepared (svr_state (svrs s svr) t) \<and> 
+    v = get_val (svr_state (svrs s svr) t) \<and>
     s' = s \<lparr> svrs := (svrs s)
       (svr := svrs s svr \<lparr>
-        wtxn_state := (wtxn_state (svrs s svr))(t := Commit cts v {} deps),
-        clock := Suc (max (clock (svrs s svr)) (cl_clock (cls s (get_cl_w t)))),
-        lst := if pending_wtxns_ts ((wtxn_state (svrs s svr)) (t := Commit cts v {} deps)) = {}
-               then clock (svrs s svr)
-               else Min (pending_wtxns_ts ((wtxn_state (svrs s svr)) (t := Commit cts v {} deps)))
+        svr_state := (svr_state (svrs s svr))(t := Commit cts v {} deps),
+        svr_clock := Suc (max (svr_clock (svrs s svr)) (cl_clock (cls s (get_cl_w t)))),
+        lst := if pending_wtxns_ts ((svr_state (svrs s svr)) (t := Commit cts v {} deps)) = {}
+               then svr_clock (svrs s svr)
+               else Min (pending_wtxns_ts ((svr_state (svrs s svr)) (t := Commit cts v {} deps)))
       \<rparr>)
     \<rparr>"
 
 
 subsection \<open>The Event System\<close>
 
-definition state_init :: "'v state" where
+definition state_init :: "'v global_conf" where
   "state_init \<equiv> \<lparr> 
-    cls = (\<lambda>cl. \<lparr> txn_state = Idle,
-                  txn_sn = 0,
-                  gst = 0,
-                  lst_map = (\<lambda>svr. 0),
+    cls = (\<lambda>cl. \<lparr> cl_state = Idle,
+                  cl_sn = 0,
+                  cl_clock = 0,
                   cl_ctx = dep_set_init,
-                  cl_clock = 0 \<rparr>),
-    svrs = (\<lambda>svr. \<lparr> wtxn_state = (\<lambda>t. No_Ver) (T0 := Commit 0 undefined {} {}),
-                    clock = 0,
+                  gst = 0,
+                  lst_map = (\<lambda>svr. 0) \<rparr>),
+    svrs = (\<lambda>svr. \<lparr> svr_state = (\<lambda>t. No_Ver) (T0 := Commit 0 undefined {} {}),
+                    svr_clock = 0,
                     lst = 0 \<rparr>),
-    commit_order = (\<lambda>k. [T0]),
     rtxn_rts = Map.empty,
-    wtxn_cts = Map.empty (T0 \<mapsto> 0)
+    wtxn_cts = Map.empty (T0 \<mapsto> 0),
+    commit_order = (\<lambda>k. [T0])
   \<rparr>"
 
-fun state_trans :: "'v state \<Rightarrow> 'v ev \<Rightarrow> 'v state \<Rightarrow> bool" where
+fun state_trans :: "'v global_conf \<Rightarrow> 'v ev \<Rightarrow> 'v global_conf \<Rightarrow> bool" where
   "state_trans s (RInvoke cl keys)          s' \<longleftrightarrow> read_invoke cl keys s s'" |
   "state_trans s (Read cl k v t)            s' \<longleftrightarrow> read cl k v t s s'" |
   "state_trans s (RDone cl kvt_map sn u'')  s' \<longleftrightarrow> read_done cl kvt_map sn u'' s s'" |
@@ -334,7 +334,7 @@ fun state_trans :: "'v state \<Rightarrow> 'v ev \<Rightarrow> 'v state \<Righta
   "state_trans s (CommitW svr t v cts deps) s' \<longleftrightarrow> commit_write svr t v cts deps s s'" |
   "state_trans s Skip2 s' \<longleftrightarrow> s' = s"
 
-definition tps :: "('v ev, 'v state) ES" where
+definition tps :: "('v ev, 'v global_conf) ES" where
   "tps \<equiv> \<lparr>
     init = (=) state_init,
     trans = state_trans
@@ -350,23 +350,23 @@ lemma tps_trans [simp]: "trans tps = state_trans" by (simp add: tps_def)
 
 subsection \<open>Simulation function\<close>
 
-abbreviation is_done :: "'v state \<Rightarrow> txid0 \<Rightarrow> bool" where
-  "is_done s t \<equiv> txn_sn (cls s (get_cl t)) > get_sn t"
+abbreviation is_done :: "'v global_conf \<Rightarrow> txid0 \<Rightarrow> bool" where
+  "is_done s t \<equiv> cl_sn (cls s (get_cl t)) > get_sn t"
 
 term "Set.filter (is_done s) rs"
 
-definition kvs_of_s :: "'v state \<Rightarrow> 'v kv_store" where
+definition kvs_of_s :: "'v global_conf \<Rightarrow> 'v kv_store" where
   "kvs_of_s s \<equiv>
     (\<lambda>k. map
-      (\<lambda>t. case wtxn_state (svrs s k) t of
+      (\<lambda>t. case svr_state (svrs s k) t of
         Prep ts v \<Rightarrow> \<lparr>v_value = v, v_writer = t, v_readerset = {}\<rparr> |
         Commit cts v rs deps \<Rightarrow> \<lparr>v_value = v, v_writer = t, v_readerset = {t \<in> rs. is_done s t}\<rparr>)
       (commit_order s k))"
 
-definition views_of_s :: "'v state \<Rightarrow> (cl_id \<Rightarrow> view)" where
+definition views_of_s :: "'v global_conf \<Rightarrow> (cl_id \<Rightarrow> view)" where
   "views_of_s s = (\<lambda>cl. view_of (commit_order s) (cl_ctx (cls s cl)))"
 
-definition sim :: "'v state \<Rightarrow> 'v config" where         
+definition sim :: "'v global_conf \<Rightarrow> 'v config" where         
   "sim s = (kvs_of_s s, views_of_s s)"
 
 lemmas sim_defs = sim_def kvs_of_s_def views_of_s_def
